Imp.v
@@ -29,14 +29,11 @@ Inductive aexp : Type :=
   | AMinus : aexp -> aexp -> aexp
   | AMult : aexp -> aexp -> aexp
   | AVar :  id -> aexp 
-  | ARead : aexp -> aexp.
+  | ARead : id -> aexp.
 
-Definition idA : id := Id 0.
-Definition idB : id := Id 1.
-Definition idC : id := Id 2.
-Definition A : aexp := ANum 0.
-Definition B : aexp := ANum 1.
-Definition C : aexp := ANum 2.
+Definition A : id := Id 0.
+Definition B : id := Id 1.
+Definition C : id := Id 2.
 
 Inductive bexp : Type :=
   | BTrue : bexp
@@ -60,7 +57,7 @@ Fixpoint aeval (h : heap) (v : valuation) (a : aexp) : nat :=
    just perform lookup on different structures 
   *)                               
   | AVar x => v x
-  | ARead x => (h (Id (aeval h v x))) 
+  | ARead x => h x 
   end.
 
 Fixpoint beval (h : heap) (v : valuation) (b : bexp) : bool :=
@@ -73,8 +70,8 @@ Fixpoint beval (h : heap) (v : valuation) (b : bexp) : bool :=
   | BAnd b1 b2  => andb (beval h v b1) (beval h v b2)
   end.
 
-Compute  aeval empty_heap (t_update empty_valuation idA 5)
-        (APlus (ANum 3) (AMult (AVar idA) (ANum 2))).
+Compute  aeval empty_heap (t_update empty_valuation A 5)
+        (APlus (ANum 3) (AMult (AVar A) (ANum 2))).
 
 
 (* ################################################################# *)
@@ -87,7 +84,7 @@ Inductive com : Type :=
   | CIf : bexp -> com -> com -> com
   | CWhile : bexp -> com -> com
   | CVar : id -> aexp -> com
-  | CWrite : aexp -> aexp -> com.
+  | CWrite : id -> aexp -> com.
 
 Notation "'SKIP'" :=
   CSkip.
@@ -97,8 +94,8 @@ Notation "'WHILE' b 'DO' c 'END'" :=
   (CWhile b c) (at level 80, right associativity).
 Notation "'IFB' c1 'THEN' c2 'ELSE' c3 'FI'" :=
   (CIf c1 c2 c3) (at level 80, right associativity).
-Notation "a1 '**=' a2" :=
-  (CWrite a1 a2) (at level 60).
+Notation "'[*' x ']'  '::=' a" :=
+  (CWrite x a) (at level 60).
 Notation "x '::=' a" :=
   (CVar x a) (at level 60).
 
@@ -131,31 +128,30 @@ Inductive ceval : heap -> valuation -> com -> heap -> valuation -> Prop :=
   | E_Var  : forall (h : heap) (v : valuation) (a1 : aexp) (n : nat) (x : id),
       aeval h v a1 = n ->
       ceval h v (x ::= a1) h (t_update v x n)
-  | E_Write : forall (h : heap) (v : valuation) (a1 a2 : aexp) (n n' : nat),
+  | E_Write : forall (h : heap) (v : valuation) (x : id) ( a1 : aexp) (n : nat),
       aeval h v a1 = n ->
-      aeval h v a2 = n' ->
-      ceval h v (a1 **= a2) (t_update h (Id n) n') v.
+      ceval h v ( [*x] ::= a1) (t_update h x n) v.
 
 
 
 
 Example ex_cwrite :  ceval empty_heap empty_valuation
-                           (A **= (APlus (ANum 3) (ANum 12)))
-                           (t_update empty_heap idA 15) empty_valuation.
+                           ( [*A] ::= (APlus (ANum 3) (ANum 12)))
+                           (t_update empty_heap A 15) empty_valuation.
 Proof.
   simpl. apply E_Write; auto. Qed.
 
 Example ex_complex :
   ceval
     empty_heap empty_valuation
-    (A **= ANum 2;;
+    ([*A] ::= ANum 2;;
      IFB BEq (ARead A) (ANum 2)
-       THEN B **= ANum 3
-       ELSE C **= ANum 4
+       THEN [*B] ::= ANum 3
+       ELSE [*C] ::= ANum 4
      FI)     
-     (t_update (t_update empty_heap idA 2) idB 3) empty_valuation.
+     (t_update (t_update empty_heap A 2) B 3) empty_valuation.
 Proof.
-  apply E_Seq with (t_update empty_heap (Id 0) 2) empty_valuation.
+  apply E_Seq with (t_update empty_heap A 2) empty_valuation.
   - constructor; auto.
   - repeat constructor; auto.
 Qed.
@@ -165,30 +161,30 @@ Qed.
    [X] (inclusive: [1 + 2 + ... + X]) in the variable [Y]. *)
    
 Definition pup_to_n : com :=
-  B **= ANum 0;;  
+  [*B] ::= ANum 0;;  
   WHILE (BNot (BEq (ANum 0) (ARead A))) DO
   (
-    B **= APlus (ARead B) (ARead A);;
-    A **= AMinus (ARead A) (ANum 1)
+    [*B] ::= APlus (ARead B) (ARead A);;
+    [*A] ::= AMinus (ARead A) (ANum 1)
   )
   END.
 
 (* Proof that this program executes as intended for [X] = [2] *)
 Theorem pup_to_2_ceval :
-  ceval (t_update empty_heap idA 2) empty_valuation
+  ceval (t_update empty_heap A 2) empty_valuation
   pup_to_n  
-  (t_update (t_update (t_update (t_update (t_update (t_update empty_heap idA 2) idB 0) idB 2) idA 1) idB 3) idA 0) empty_valuation.
+  (t_update (t_update (t_update (t_update (t_update (t_update empty_heap A 2) B 0) B 2) A 1) B 3) A 0) empty_valuation.
 Proof.
-  apply E_Seq with (h2 := (t_update (t_update empty_heap idA 2) idB 0) ) (v2 := empty_valuation).
+  apply E_Seq with (h2 := (t_update (t_update empty_heap A 2) B 0) ) (v2 := empty_valuation).
   - constructor; auto. 
-  - apply E_WhileLoop  with (h2 := (t_update (t_update (t_update (t_update empty_heap idA 2) idB 0) idB 2) idA 1))
+  - apply E_WhileLoop  with (h2 := (t_update (t_update (t_update (t_update empty_heap A 2) B 0) B 2) A 1))
                            (v2 := empty_valuation).
     + auto.
-    + apply E_Seq with (h2 := (t_update (t_update (t_update empty_heap idA 2) idB 0) idB 2))
+    + apply E_Seq with (h2 := (t_update (t_update (t_update empty_heap A 2) B 0) B 2))
                          (v2 := empty_valuation); apply E_Write; auto; constructor.
-    + apply E_WhileLoop with (h2 :=  (t_update (t_update (t_update (t_update (t_update (t_update empty_heap idA 2) idB 0) idB 2) idA 1) idB 3) idA 0)) (v2 := empty_valuation).
+    + apply E_WhileLoop with (h2 :=  (t_update (t_update (t_update (t_update (t_update (t_update empty_heap A 2) B 0) B 2) A 1) B 3) A 0)) (v2 := empty_valuation).
       * auto.
-      * apply E_Seq with (h2 := (t_update (t_update (t_update (t_update (t_update empty_heap idA 2) idB 0) idB 2) idA 1) idB 3)) (v2 := empty_valuation);
+      * apply E_Seq with (h2 := (t_update (t_update (t_update (t_update (t_update empty_heap A 2) B 0) B 2) A 1) B 3)) (v2 := empty_valuation);
         apply E_Write; auto; constructor.
       * apply E_WhileEnd. auto.
 Qed.       
@@ -199,7 +195,6 @@ Qed.
 
 (* $Date: 2016-07-18 $ *)
 
-(* TODO We shouldn't need to typecast an aexp into an id everytime we add or look-up a key in a heap *)
 (* TODO Some notational sugar for the map types (I mean, just look at the last proof) *)
 (* TODO Find a way to represent heap and valuation as one st object - Its getting tedious*)
 
